aarch64 refine: ArchAcc_R sorry free
Signed-off-by: Gerwin Klein <gerwin.klein@proofcraft.systems>

proof/refine/AARCH64/ArchAcc_R.thy
@@ -391,6 +391,15 @@ lemma one_less_2p_pte_bits[simp]:
   "(1::machine_word) < 2 ^ pte_bits"
   by (simp add: bit_simps)
 
+lemma pt_apply_upd_eq':
+  "idx \<le> mask (ptTranslationBits (pt_type pt)) \<Longrightarrow>
+   pt_apply (pt_upd pt (table_index (pt_type pt) p) pte) idx =
+   (if table_index (pt_type pt) p = idx then pte else pt_apply pt idx)"
+  unfolding pt_apply_def pt_upd_def
+  using table_index_mask_eq[where pt_t=NormalPT_T] table_index_mask_eq[where pt_t=VSRootPT_T]
+  by (cases pt; clarsimp simp: ucast_eq_mask vs_index_ptTranslationBits pt_index_ptTranslationBits
+                               word_le_mask_eq)
+
 \<comment> \<open>setObject_other_corres unfortunately doesn't work here\<close>
 lemma setObject_PT_corres:
   "pte_relation' pte pte' \<Longrightarrow>
@@ -426,36 +435,25 @@ lemma setObject_PT_corres:
     apply (drule_tac x = x in bspec)
      apply simp
     apply (rule conjI; clarsimp)
-     apply (clarsimp simp: pte_relation_def)
-    prefer 2
-  sorry (* FIXME AARCH64
-    apply (clarsimp simp: pte_relation_def table_base_index_eq
+     apply (clarsimp simp: pte_relation_def pt_apply_upd_eq')
+     apply (metis more_pt_inner_beauty)
+    apply (clarsimp simp: pte_relation_def table_base_index_eq pt_apply_upd_eq'
                    dest!: more_pt_inner_beauty)
-    apply (simp add: pt_apply_pt_upd_eq)
    apply (rule ballI)
    apply (drule (1) bspec)
    apply clarsimp
    apply (rule conjI)
-    apply (clarsimp simp: pte_relation_def table_base_index_eq
-                   dest!: more_pt_inner_beauty)
+    apply (clarsimp simp: pte_relation_def pt_apply_upd_eq')
+    apply (metis more_pt_inner_beauty table_base_index_eq)
    apply clarsimp
    apply (drule bspec, assumption)
    apply clarsimp
    apply (erule (1) obj_relation_cutsE)
       apply simp
-     apply simp
      apply clarsimp
-     apply (frule (1) pspace_alignedD)
-     apply (drule_tac p=x in pspace_alignedD, assumption)
-     apply simp
-     apply (drule mask_alignment_ugliness)
-        apply (simp add: pt_bits_def pageBits_def)
-       apply (simp add: pt_bits_def pageBits_def)
-      apply clarsimp
-      apply (drule test_bit_size)
-      apply (clarsimp simp: word_size bit_simps)
-      apply arith
-     apply ((simp split: if_split_asm)+)[2]
+     apply (smt (verit, best) pspace_aligned_pts_ofD pts_of_Some pts_of_type_unique aobjs_of_Some
+                              table_base_plus)
+    apply ((simp split: if_split_asm)+)[2]
    apply (simp add: other_obj_relation_def
                split: Structures_A.kernel_object.splits arch_kernel_obj.splits)
   apply (rule conjI)
@@ -470,7 +468,7 @@ lemma setObject_PT_corres:
   apply (simp add: map_to_ctes_upd_other)
   apply (simp add: fun_upd_def)
   apply (simp add: caps_of_state_after_update obj_at_def swp_cte_at_caps_of)
-  done *)
+  done
 
 lemma storePTE_corres:
   "pte_relation' pte pte' \<Longrightarrow>
@@ -503,7 +501,7 @@ lemma bit_simps_corres[simp]:
   by (simp add: bit_simps bitSimps)
 
 defs checkPTAt_def:
-  "checkPTAt p \<equiv> stateAssert (\<lambda>s. \<exists>pt_t. page_table_at' pt_t p s) []"
+  "checkPTAt p \<equiv> stateAssert (\<lambda>s. \<exists>pt. page_table_at' pt p s) []"
 
 lemma pte_relation_must_pte:
   "pte_relation m (ArchObj (PageTable pt)) ko \<Longrightarrow> \<exists>pte. ko = (KOArch (KOPTE pte))"
@@ -603,9 +601,12 @@ lemma user_region_or:
   "\<lbrakk> vref \<in> user_region; vref' \<in> user_region \<rbrakk> \<Longrightarrow> vref || vref' \<in> user_region"
   by (simp add: user_region_def canonical_user_def le_mask_high_bits word_size)
 
+lemma gets_the_oapply2_comp: (* FIXME AARCH64: move to OptionMonad *)
+  "gets_the (oapply2 y x \<circ> f) = gets_map (swp f y) x"
+  by (clarsimp simp: gets_map_def gets_the_def o_def gets_def)
 
 lemma lookupPTSlotFromLevel_corres:
-  "\<lbrakk> level' = size level; pt' = pt \<rbrakk> \<Longrightarrow>
+  "\<lbrakk> level' = size level; pt' = pt; level \<le> max_pt_level \<rbrakk> \<Longrightarrow>
    corres (\<lambda>(level, p) (bits, p'). bits = pt_bits_left level \<and> p' = p)
      (pspace_aligned and pspace_distinct and valid_vspace_objs and valid_asid_table and
      \<exists>\<rhd> (level, pt) and K (vptr \<in> user_region \<and> level \<le> max_pt_level))
@@ -624,27 +625,36 @@ next
   with nlevel
   have level: "size level = Suc (size nlevel)" by simp
 
+  from `0 < level` `level \<le> max_pt_level`
+  have level_m1: "level - 1 \<le> max_pt_level"
+    by blast
+
+  from level
+  have levelType[simp]:
+    "levelType (Suc (size nlevel)) = level_type level"
+    unfolding levelType_def using vm_level.size_inj
+    by fastforce
+
   define vref_step where
-    "vref_step vref \<equiv>
-       vref_for_level vref (level+1) || (pt_index level vptr << pt_bits_left level)"
+    "vref_step vref \<equiv> vref_for_level vref (level+1) || (pt_index level vptr << pt_bits_left level)"
     for vref
 
+  from `level \<le> max_pt_level`
   have vref_for_level_step[simp]:
-    "level \<le> max_pt_level \<Longrightarrow>
-     vref_for_level (vref_step vref) (level + 1) = vref_for_level vref (level + 1)"
+    "vref_for_level (vref_step vref) (level + 1) = vref_for_level vref (level + 1)"
     for vref
     unfolding vref_step_def
     using vref_for_level_pt_index_idem[of level level level vref vptr] by simp
 
+  from `level \<le> max_pt_level`
   have pt_walk_vref[simp]:
-    "level \<le> max_pt_level \<Longrightarrow>
-     pt_walk max_pt_level level pt (vref_step vref) =
+    "pt_walk max_pt_level level pt (vref_step vref) =
      pt_walk max_pt_level level pt vref" for pt vref
-    by (rule pt_walk_vref_for_level_eq; simp)
+    by - (rule pt_walk_vref_for_level_eq; simp)
 
+  from `level \<le> max_pt_level`
   have vref_step_user_region[simp]:
-    "\<lbrakk> vref \<in> user_region; vptr \<in> user_region; level \<le> max_pt_level \<rbrakk>
-     \<Longrightarrow> vref_step vref \<in> user_region"
+    "\<lbrakk> vref \<in> user_region; vptr \<in> user_region \<rbrakk> \<Longrightarrow> vref_step vref \<in> user_region"
     for vref
     unfolding vref_step_def
     using nlevel1 nlevel
@@ -657,43 +667,66 @@ next
     "\<lbrakk> is_aligned pt (pt_bits level); vref \<in> user_region \<rbrakk> \<Longrightarrow>
      pt_slot_offset level pt (vref_step vref) = pt_slot_offset level pt vptr" for vref
     unfolding vref_step_def using nlevel1 nlevel
-    sorry (* FIXME AARCH64
-    by (auto simp: pt_slot_offset_or_def user_region_def canonical_user_def
-                   word_eqI_simps pt_index_def bit_simps pt_bits_left_def
-             dest!: max_pt_level_enum
-             intro!: word_eqI) *)
+    apply simp
+    apply (clarsimp simp: pt_slot_offset_or_def user_region_def canonical_user_def)
+    apply (simp add: pt_index_def pt_bits_left_def)
+    apply (rule conjI; clarsimp)
+     apply (simp add: plus_one_eq_asid_pool vref_for_level_def pt_bits_left_def)
+     apply (rule conjI, simp add: max_pt_level_def)
+     apply (clarsimp simp: level_defs bit_simps maxPTLevel_def)
+     apply word_eqI_solve
+    apply (clarsimp simp: vref_for_level_def pt_bits_left_def)
+    apply (rule conjI; clarsimp)
+     apply (subgoal_tac "nlevel = max_pt_level - 1")
+      apply (clarsimp simp: level_defs bit_simps maxPTLevel_def split: if_split_asm)
+      apply word_eqI_solve
+     apply (subst (asm) add.commute[where a=2])
+     apply (drule add_implies_diff)
+     apply (simp add: max_pt_level_def)
+    apply (simp add: pt_bits_def)
+    apply (prop_tac "level_type (nlevel + 1) = NormalPT_T")
+     apply (drule max_pt_level_enum)
+     apply (auto simp: level_defs split: if_split_asm)[1]
+    apply (simp add: bit_simps)
+    apply word_eqI
+    apply (drule max_pt_level_enum)
+    by (auto split: if_split_asm)
 
-  from `0 < level` `level' = size level` `pt' = pt` level
+  from `0 < level` `level' = size level` `pt' = pt` level `level \<le> max_pt_level` level_m1
   show ?case
     apply (subst pt_lookup_slot_from_level_rec)
     apply (simp add: lookupPTSlotFromLevel.simps Let_def obind_comp_dist if_comp_dist
-                     gets_the_if_distrib checkPTAt_def)
-    sorry (* FIXME AARCH64
+                     gets_the_if_distrib checkPTAt_def gets_the_oapply2_comp)
     apply (rule corres_guard_imp, rule corres_split[where r'=pte_relation'])
          apply (rule pteAtIndex_corres, simp)
         apply (rule corres_if3)
           apply (rename_tac pte pte', case_tac pte; (simp add: isPageTablePTE_def))
          apply (rule corres_stateAssert_implied)
           apply (rule minus(1))
-           apply (simp add: nlevel)
-          apply (clarsimp simp: AARCH64_A.is_PageTablePTE_def pptr_from_pte_def getPPtrFromHWPTE_def
-                                addr_from_ppn_def)
+            apply (simp add: nlevel)
+           apply (clarsimp simp: AARCH64_A.is_PageTablePTE_def pptr_from_pte_def getPPtrFromPTE_def
+                                 paddr_from_ppn_def isPagePTE_def)
+          apply simp
          apply clarsimp
+         apply (rule_tac x=NormalPT_T in exI)
          apply (rule page_table_at_cross; assumption?)
           apply (drule (2) valid_vspace_objs_strongD; assumption?)
            apply simp
           apply (clarsimp simp: pt_at_eq in_omonad AARCH64_A.is_PageTablePTE_def pptr_from_pte_def
-                                getPPtrFromHWPTE_def addr_from_ppn_def)
+                                getPPtrFromPTE_def isPagePTE_def paddr_from_ppn_def)
          apply (simp add: state_relation_def)
         apply (rule corres_inst[where P=\<top> and P'=\<top>])
         apply (clarsimp simp: ptSlotIndex_def pt_slot_offset_def pt_index_def pt_bits_left_def
                               ptIndex_def ptBitsLeft_def)
+        apply (rule conjI; clarsimp)
+        apply (metis vm_level.size_less_eq size_maxPTLevel)
        apply wpsimp+
      apply (frule (5) vs_lookup_table_is_aligned)
      apply (rule conjI)
       apply (drule (5) valid_vspace_objs_strongD)
-      apply (clarsimp simp: pte_at_def obj_at_def elim!: opt_mapE)
+      apply (clarsimp simp: pte_at_def obj_at_def ptes_of_def in_omonad)
       apply (simp add: pt_slot_offset_def)
+      apply (rule conjI, fastforce)
       apply (rule is_aligned_add)
        apply (erule is_aligned_weaken)
        apply (simp add: bit_simps)
@@ -705,12 +738,12 @@ next
      apply (rule conjI)
       apply (clarsimp simp: level_defs)
      apply (subst pt_walk_split_Some[where level'=level]; simp?)
-      apply (drule bit0.pred)
+      apply (drule vm_level.pred)
       apply simp
      apply (subst pt_walk.simps)
      apply (simp add: in_omonad)
     apply simp
-    done *)
+    done
 qed
 
 lemma lookupPTSlot_corres:
@@ -751,7 +784,7 @@ next
   from `0 < level`
   obtain nlevel where nlevel: "level = nlevel + 1" by (auto intro: that[of "level-1"])
   with `0 < level`
-  have nlevel1: "nlevel < nlevel + 1" using bit1.pred by fastforce
+  have nlevel1: "nlevel < nlevel + 1" using vm_level.pred by fastforce
   with nlevel
   have level: "size level = Suc (size nlevel)" by simp
 
@@ -788,13 +821,32 @@ next
     "\<lbrakk> is_aligned pt (pt_bits level); vref \<in> user_region \<rbrakk> \<Longrightarrow>
     pt_slot_offset level pt (vref_step vref) = pt_slot_offset level pt vptr" for vref
     unfolding vref_step_def using nlevel1 nlevel
-    sorry (* FIXME AARCH64
-    by (auto simp: pt_slot_offset_or_def user_region_def canonical_user_def
-                   word_eqI_simps pt_index_def bit_simps pt_bits_left_def
-             dest!: max_pt_level_enum
-             intro!: word_eqI) *)
+    apply simp
+    apply (clarsimp simp: pt_slot_offset_or_def user_region_def canonical_user_def)
+    apply (simp add: pt_index_def pt_bits_left_def)
+    apply (rule conjI; clarsimp)
+     apply (simp add: plus_one_eq_asid_pool vref_for_level_def pt_bits_left_def)
+     apply (rule conjI, simp add: max_pt_level_def)
+     apply (clarsimp simp: level_defs bit_simps maxPTLevel_def)
+     apply word_eqI_solve
+    apply (clarsimp simp: vref_for_level_def pt_bits_left_def)
+    apply (rule conjI; clarsimp)
+     apply (subgoal_tac "nlevel = max_pt_level - 1")
+      apply (clarsimp simp: level_defs bit_simps maxPTLevel_def split: if_split_asm)
+      apply word_eqI_solve
+     apply (subst (asm) add.commute[where a=2])
+     apply (drule add_implies_diff)
+     apply (simp add: max_pt_level_def)
+    apply (simp add: pt_bits_def)
+    apply (prop_tac "level_type (nlevel + 1) = NormalPT_T")
+     apply (drule max_pt_level_enum)
+     apply (auto simp: level_defs split: if_split_asm)[1]
+    apply (simp add: bit_simps)
+    apply word_eqI
+    apply (drule max_pt_level_enum)
+    by (auto split: if_split_asm)
 
-  note bit1.size_minus_one[simp]
+  note vm_level.size_minus_one[simp]
   from minus.prems
   show ?case
     apply (subst lookupPTFromLevel.simps, subst pt_lookup_from_level_simps)
@@ -808,28 +860,30 @@ next
           apply (simp add: lookup_failure_map_def)
          apply (rename_tac pte pte', case_tac pte; simp add: isPageTablePTE_def)
         apply (rule corres_if)
-    sorry (* FIXME AARCH64
-          apply (clarsimp simp: AARCH64_A.is_PageTablePTE_def pptr_from_pte_def getPPtrFromHWPTE_def
-                                addr_from_ppn_def)
-         apply (rule corres_returnOk[where P=\<top> and P'=\<top>], rule refl)
+          apply (clarsimp simp: AARCH64_A.is_PageTablePTE_def pptr_from_pte_def getPPtrFromPTE_def
+                                paddr_from_ppn_def isPagePTE_def)
+         apply (rule corres_returnOk[where P=\<top> and P'=\<top>], simp)
         apply (clarsimp simp: checkPTAt_def)
         apply (subst liftE_bindE, rule corres_stateAssert_implied)
          apply (rule minus.hyps)
           apply (simp add: minus.hyps(2))
-         apply (clarsimp simp: AARCH64_A.is_PageTablePTE_def pptr_from_pte_def getPPtrFromHWPTE_def
-                               addr_from_ppn_def)
+         apply (clarsimp simp: AARCH64_A.is_PageTablePTE_def pptr_from_pte_def getPPtrFromPTE_def
+                               paddr_from_ppn_def isPagePTE_def)
         apply clarsimp
+        apply (rule_tac x=NormalPT_T in exI)
         apply (rule page_table_at_cross; assumption?)
          apply (drule vs_lookup_table_pt_at; simp?)
-         apply (clarsimp simp: AARCH64_A.is_PageTablePTE_def pptr_from_pte_def getPPtrFromHWPTE_def
-                               addr_from_ppn_def)
+         apply (clarsimp simp: AARCH64_A.is_PageTablePTE_def pptr_from_pte_def getPPtrFromPTE_def
+                               paddr_from_ppn_def isPagePTE_def)
+         apply (simp add: level_type_def split: if_split_asm)
         apply (simp add: state_relation_def)
        apply wpsimp+
-     apply (simp add: bit0.neq_0_conv)
+     apply (simp add: vm_level.neq_0_conv)
      apply (frule (5) vs_lookup_table_is_aligned)
      apply (rule conjI)
       apply (drule (5) valid_vspace_objs_strongD)
-      apply (clarsimp simp: pte_at_def obj_at_def elim!: opt_mapE)
+      apply (clarsimp simp: pte_at_def obj_at_def ptes_of_def in_omonad)
+      apply (rule conjI, fastforce)
       apply (simp add: pt_slot_offset_def)
       apply (rule is_aligned_add)
        apply (erule is_aligned_weaken)
@@ -842,12 +896,12 @@ next
      apply (rule conjI)
       apply (clarsimp simp: level_defs)
      apply (subst pt_walk_split_Some[where level'=level]; simp?)
-      apply (drule bit0.pred)
+      apply (drule vm_level.pred)
       apply simp
      apply (subst pt_walk.simps)
      apply (simp add: in_omonad)
     apply wpsimp
-    done *)
+    done
 qed
 
 declare in_set_zip_refl[simp]
@@ -1038,6 +1092,17 @@ lemma getASIDPoolEntry_corres:
   apply simp
   done
 
+lemma no_0_page_table:
+  "\<lbrakk> no_0_obj' s; page_table_at' pt_t 0 s \<rbrakk> \<Longrightarrow> False"
+  apply (clarsimp simp: page_table_at'_def)
+  apply (erule_tac x=0 in allE)
+  apply simp
+  done
+
+crunches getASIDPoolEntry
+  for no_0_obj'[wp]: no_0_obj'
+  (wp: getObject_inv simp: loadObject_default_def)
+
 lemma findVSpaceForASID_corres:
   assumes "asid' = ucast asid"
   shows "corres (lfr \<oplus> (=))
@@ -1055,58 +1120,31 @@ lemma findVSpaceForASID_corres:
     apply (rule corres_initial_splitE[where r'="\<lambda>r r'. r = map_option abs_asid_entry r'"])
        apply simp
        apply (rule getASIDPoolEntry_corres)
-  sorry (* FIXME AARCH64: old proof below from RISCV64
-
-  using assms
-  apply (simp add: findVSpaceForASID_def)
-  apply (rule corres_gen_asm, simp add: ucast_down_ucast_id is_down_def target_size source_size)
-  apply (rule corres_guard_imp[where Q'="?Q"], rule monadic_rewrite_corres_l[where P="?P"],
-         rule find_vspace_for_asid_rewite; simp)
-  apply (simp add: liftE_bindE asidRange_def flip: mask_2pm1)
-  apply (rule_tac r'="\<lambda>x y. x = y o ucast"
-             in corres_underlying_split [OF _ _ gets_sp gets_sp])
-   apply (clarsimp simp: state_relation_def arch_state_relation_def)
-  apply (case_tac "rv (asid_high_bits_of asid)")
-   apply (simp add: liftME_def lookup_failure_map_def)
-  apply (simp add: liftME_def bindE_assoc)
-  apply (simp add: liftE_bindE)
-  apply (rule corres_guard_imp)
-    apply (rule corres_split[OF getObject_ASIDPool_corres[OF refl]])
-      apply (rule_tac P="case_option \<top> pt_at (pool (ucast asid)) and pspace_aligned and pspace_distinct"
-                 and P'="no_0_obj'" in corres_inst)
-      apply (rule_tac F="pool (ucast asid) \<noteq> Some 0" in corres_req)
-       apply (clarsimp simp: obj_at_def no_0_obj'_def state_relation_def
-                             pspace_relation_def a_type_def)
-       apply (simp split: Structures_A.kernel_object.splits
-                          arch_kernel_obj.splits if_split_asm)
-       apply (drule_tac f="\<lambda>S. 0 \<in> S" in arg_cong)
-       apply (simp add: pspace_dom_def)
-       apply (drule iffD1, rule rev_bexI, erule domI)
-        apply simp
-        apply (rule image_eqI[rotated])
-         apply (rule rangeI[where x=0])
-        apply simp
-       apply clarsimp
-      apply (simp add: mask_asid_low_bits_ucast_ucast asid_low_bits_of_def returnOk_def
-                       lookup_failure_map_def ucast_ucast_a is_down
-                  split: option.split)
-      apply clarsimp
-      apply (simp add: returnOk_liftE checkPTAt_def liftE_bindE)
-      apply (rule corres_stateAssert_implied[where P=\<top>, simplified])
-       apply simp
-      apply clarsimp
-      apply (rule page_table_at_cross; assumption?)
-      apply fastforce
-     apply (wp getObject_inv loadObject_default_inv | simp)+
-   apply (clarsimp simp: o_def)
-   apply (rule conjI)
-    apply (rule valid_asid_tableD; simp)
-   apply (clarsimp split: option.splits)
-   apply (rule vs_lookup_table_pt_at[where vptr=0 and level=max_pt_level and asid=asid]; simp?)
-   apply (simp add: vs_lookup_table_def pool_for_asid_def vspace_for_pool_def in_omonad obj_at_def
-                    asid_low_bits_of_def)
-  apply simp
-  done *)
+      apply (rule_tac Q="\<lambda>entry s. pspace_aligned s \<and> pspace_distinct s \<and>
+                                   vspace_pt_at (ap_vspace entry) s"
+                      in option_corres[where P=\<top> and P'=\<top> and Q'="\<lambda>_. no_0_obj'"])
+        apply (clarsimp simp: lookup_failure_map_def)
+       apply (rename_tac entry entry')
+       apply (case_tac entry')
+       apply (clarsimp simp: checkPTAt_def abs_asid_entry_def)
+       apply (rename_tac p)
+       apply (rule_tac Q="\<lambda>s. \<exists>pt_t. page_table_at' pt_t p s \<and> no_0_obj' s" in corres_cross_over_guard)
+        apply clarsimp
+        apply (rule_tac x=VSRootPT_T in exI)
+        apply (erule (2) page_table_at_cross, simp add: state_relation_def)
+       apply (simp add: liftE_bindE assertE_liftE)
+       apply (rule corres_assert_assume)
+        apply (rule corres_stateAssert_assume)
+         apply (rule corres_returnOk, simp)
+        apply clarsimp
+       apply (fastforce dest: no_0_page_table)
+      apply simp
+     apply wpsimp
+     apply (clarsimp simp: entry_for_asid_def)
+     apply (drule (2) pool_for_asid_valid_vspace_objs)
+     apply (fastforce simp: entry_for_pool_def)
+    apply (wpsimp wp: hoare_drop_imps)+
+  done
 
 lemma setObject_arch:
   assumes X: "\<And>p q n ko. \<lbrace>\<lambda>s. P (ksArchState s)\<rbrace> updateObject val p q n ko \<lbrace>\<lambda>rv s. P (ksArchState s)\<rbrace>"
